{
  "@context": {
    "id": "@id",
    "type": "@type",
    "dc:title": {
      "@container": "@language"
    },
    "dc:description": {
      "@container": "@language"
    },
    "rdfs:comment": {
      "@container": "@language"
    },
    "rdfs:domain": {
      "@type": "@id"
    },
    "rdfs:label": {
      "@container": "@language"
    },
    "rdfs:range": {
      "@type": "@id"
    },
    "rdfs:subClassOf": {
      "@type": "@id"
    },
    "rdfs:subPropertyOf": {
      "@type": "@id"
    },
    "owl:equivalentClass": {
      "@type": "@vocab"
    },
    "owl:equivalentProperty": {
      "@type": "@vocab"
    },
    "owl:oneOf": {
      "@container": "@list",
      "@type": "@vocab"
    },
    "owl:imports": {
      "@type": "@id"
    },
    "owl:versionInfo": {
      "@type": "xsd:string",
      "@language": null
    },
    "owl:inverseOf": {
      "@type": "@vocab"
    },
    "owl:unionOf": {
      "@type": "@vocab",
      "@container": "@list"
    },
    "rdfs_classes": {
      "@reverse": "rdfs:isDefinedBy",
      "@type": "@id"
    },
    "rdfs_properties": {
      "@reverse": "rdfs:isDefinedBy",
      "@type": "@id"
    },
    "rdfs_datatypes": {
      "@reverse": "rdfs:isDefinedBy",
      "@type": "@id"
    },
    "rdfs_instances": {
      "@reverse": "rdfs:isDefinedBy",
      "@type": "@id"
    },
    "cc": "http://creativecommons.org/ns#",
    "csvw": "http://www.w3.org/ns/csvw#",
    "ctag": "http://commontag.org/ns#",
    "dc": "http://purl.org/dc/terms/",
    "dc11": "http://purl.org/dc/elements/1.1/",
    "dcat": "http://www.w3.org/ns/dcat#",
    "dcterms": "http://purl.org/dc/terms/",
    "foaf": "http://xmlns.com/foaf/0.1/",
    "gr": "http://purl.org/goodrelations/v1#",
    "grddl": "http://www.w3.org/2003/g/data-view#",
    "ical": "http://www.w3.org/2002/12/cal/icaltzd#",
    "ma": "http://www.w3.org/ns/ma-ont#",
    "og": "http://ogp.me/ns#",
    "org": "http://www.w3.org/ns/org#",
    "owl": "http://www.w3.org/2002/07/owl#",
    "prov": "http://www.w3.org/ns/prov#",
    "qb": "http://purl.org/linked-data/cube#",
    "rdf": "http://www.w3.org/1999/02/22-rdf-syntax-ns#",
    "rdfa": "http://www.w3.org/ns/rdfa#",
    "rdfs": "http://www.w3.org/2000/01/rdf-schema#",
    "rev": "http://purl.org/stuff/rev#",
    "rif": "http://www.w3.org/2007/rif#",
    "rr": "http://www.w3.org/ns/r2rml#",
    "schema": "http://schema.org/",
    "sd": "http://www.w3.org/ns/sparql-service-description#",
    "sioc": "http://rdfs.org/sioc/ns#",
    "skos": "http://www.w3.org/2004/02/skos/core#",
    "skosxl": "http://www.w3.org/2008/05/skos-xl#",
    "v": "http://rdf.data-vocabulary.org/#",
    "vcard": "http://www.w3.org/2006/vcard/ns#",
    "void": "http://rdfs.org/ns/void#",
    "wdr": "http://www.w3.org/2007/05/powder#",
    "wrds": "http://www.w3.org/2007/05/powder-s#",
    "xhv": "http://www.w3.org/1999/xhtml/vocab#",
    "xml": "rdf:XMLLiteral",
    "xsd": "http://www.w3.org/2001/XMLSchema#",
    "any": "xsd:anySimpleType",
    "binary": "xsd:base64Binary",
    "datetime": "xsd:dateTime",
    "describedby": "wrds:describedby",
    "html": "rdf:HTML",
    "license": "xhv:license",
    "maximum": "csvw:maxInclusive",
    "minimum": "csvw:minInclusive",
    "number": "xsd:double",
    "role": "xhv:role",
    "anySimpleType": "xsd:anySimpleType",
    "string": "xsd:string",
    "normalizedString": "xsd:normalizedString",
    "token": "xsd:token",
    "Name": "xsd:Name",
    "NCName": "xsd:NCName",
    "boolean": "xsd:boolean",
    "lang": "xsd:language",
    "decimal": "xsd:decimal",
    "integer": "xsd:integer",
    "nonPositiveInteger": "xsd:nonPositiveInteger",
    "negativeInteger": "xsd:negativeInteger",
    "long": "xsd:long",
    "int": "xsd:int",
    "short": "xsd:short",
    "byte": "xsd:byte",
    "nonNegativeInteger": "xsd:nonNegativeInteger",
    "unsignedLong": "xsd:unsignedLong",
    "unsignedInt": "xsd:unsignedInt",
    "unsignedShort": "xsd:unsignedShort",
    "unsignedByte": "xsd:unsignedByte",
    "positiveInteger": "xsd:positiveInteger",
    "float": "xsd:float",
    "double": "xsd:double",
    "duration": "xsd:duration",
    "dateTime": "xsd:dateTime",
    "time": "xsd:time",
    "date": "xsd:date",
    "gYearMonth": "xsd:gYearMonth",
    "gYear": "xsd:gYear",
    "gMonthDay": "xsd:gMonthDay",
    "gDay": "xsd:gDay",
    "gMonth": "xsd:gMonth",
    "hexBinary": "xsd:hexBinary",
    "base64Binary": "xsd:base64Binary",
    "anyURI": "xsd:anyURI",
    "Column": "csvw:Column",
    "Dialect": "csvw:Dialect",
    "Direction": "csvw:Direction",
    "Schema": "csvw:Schema",
    "Table": "csvw:Table",
    "TableGroup": "csvw:TableGroup",
    "Template": "csvw:Template",
    "aboutUrl": {
      "@id": "csvw:aboutUrl",
      "@type": "@id"
    },
    "columns": {
      "@id": "csvw:columns",
      "@type": "@id",
      "@container": "@list"
    },
    "commentPrefix": {
      "@id": "csvw:commentPrefix",
      "@language": null
    },
    "datatype": {
      "@id": "csvw:datatype",
      "@type": "@vocab"
    },
    "default": {
      "@id": "csvw:default",
      "@language": null
    },
    "delimiter": {
      "@id": "csvw:delimiter",
      "@language": null
    },
    "dialect": {
      "@id": "csvw:dialect",
      "@type": "@id"
    },
    "doubleQuote": {
      "@id": "csvw:doubleQuote",
      "@type": "xsd:boolean"
    },
    "encoding": {
      "@id": "csvw:encoding",
      "@language": null
    },
    "foreignKeys": {
      "@id": "csvw:foreignKeys",
      "@language": null
    },
    "format": {
      "@id": "csvw:format",
      "@language": null
    },
    "header": {
      "@id": "csvw:header",
      "@type": "xsd:boolean"
    },
    "headerColumnCount": {
      "@id": "csvw:headerColumnCount",
      "@type": "xsd:nonNegativeInteger"
    },
    "headerRowCount": {
      "@id": "csvw:headerRowCount",
      "@type": "xsd:nonNegativeInteger"
    },
    "language": {
      "@id": "csvw:language",
      "@language": null
    },
    "length": {
      "@id": "csvw:length",
      "@type": "xsd:nonNegativeInteger"
    },
    "lineTerminator": {
      "@id": "csvw:lineTerminator",
      "@language": null
    },
    "maxExclusive": {
      "@id": "csvw:maxExclusive",
      "@type": "xsd:integer"
    },
    "maxInclusive": {
      "@id": "csvw:maxInclusive",
      "@type": "xsd:integer"
    },
    "maxLength": {
      "@id": "csvw:maxLength",
      "@type": "xsd:nonNegativeInteger"
    },
    "minExclusive": {
      "@id": "csvw:minExclusive",
      "@type": "xsd:integer"
    },
    "minInclusive": {
      "@id": "csvw:minInclusive",
      "@type": "xsd:integer"
    },
    "minLength": {
      "@id": "csvw:minLength",
      "@type": "xsd:nonNegativeInteger"
    },
    "name": {
      "@id": "csvw:name",
      "@language": null
    },
    "notes": {
      "@id": "csvw:notes"
    },
    "null": {
      "@id": "csvw:null",
      "@language": null
    },
    "primaryKey": {
      "@id": "csvw:primaryKey",
      "@language": null
    },
    "propertyUrl": {
      "@id": "csvw:propertyUrl",
      "@type": "@id"
    },
    "quoteChar": {
      "@id": "csvw:quoteChar",
      "@language": null
    },
    "required": {
      "@id": "csvw:required",
      "@type": "xsd:boolean"
    },
    "resources": {
      "@id": "csvw:resources",
      "@type": "@id",
      "@container": "@set"
    },
    "row": {
      "@id": "csvw:row",
      "@container": "@set"
    },
    "separator": {
      "@id": "csvw:separator",
      "@language": null
    },
    "skipBlankRows": {
      "@id": "csvw:skipBlankRows",
      "@type": "xsd:boolean"
    },
    "skipColumns": {
      "@id": "csvw:skipColumns",
      "@type": "xsd:nonNegativeInteger"
    },
    "skipInitialSpace": {
      "@id": "csvw:skipInitialSpace",
      "@type": "xsd:boolean"
    },
    "skipRows": {
      "@id": "csvw:skipRows",
      "@type": "xsd:nonNegativeInteger"
    },
    "source": {
      "@id": "csvw:source",
      "@language": null
    },
    "table": {
      "@id": "csvw:table",
      "@type": "@id",
      "@container": "@set"
    },
    "tableDirection": {
      "@id": "csvw:tableDirection",
      "@type": "@vocab"
    },
    "tableSchema": {
      "@id": "csvw:tableSchema",
      "@type": "@id"
    },
    "targetFormat": {
      "@id": "csvw:targetFormat",
      "@type": "xsd:anyURI"
    },
    "templateFormat": {
      "@id": "csvw:templateFormat",
      "@type": "xsd:anyURI"
    },
    "templates": {
      "@id": "csvw:templates",
      "@type": "@id"
    },
    "textDirection": {
      "@id": "csvw:textDirection",
      "@type": "@vocab"
    },
    "title": {
      "@id": "csvw:title",
      "@container": "@language"
    },
    "trim": {
      "@id": "csvw:trim",
      "@type": "xsd:boolean"
    },
    "url": {
      "@id": "csvw:url",
      "@type": "xsd:anyURI"
    },
    "valueUrl": {
      "@id": "csvw:valueUrl",
      "@type": "@id"
    },
    "virtual": {
      "@id": "csvw:virtual",
      "@type": "xsd:boolean"
    },
    "JSON": "csvw:JSON",
    "uriTemplate": "csvw:uriTemplate"
  },
  "@id": "http://www.w3.org/ns/csvw#",
  "@type": "owl:Ontology",
  "dc:title": {
    "en": "CSVW Namespace Vocabulary Terms"
  },
  "dc:description": {
    "en": "This document describes the RDFS vocabulary description used in the Metadata Vocabulary for Tabular Data [[csvw-metadata]] along with the default JSON-LD Context."
  },
  "rdfs_classes": [
    {
      "@id": "csvw:Column",
      "@type": "rdfs:Class",
      "rdfs:label": {
        "en": "Column Description"
      },
      "rdfs:comment": {
        "en": "A Column Description describes a single column."
      }
    },
    {
      "@id": "csvw:Dialect",
      "@type": "rdfs:Class",
      "rdfs:label": {
        "en": "Dialect Description"
      },
      "rdfs:comment": {
        "en": "A Dialect Description provides hints to parsers about how to parse a linked file."
      }
    },
    {
      "@id": "csvw:Direction",
      "@type": "rdfs:Class",
      "rdfs:label": {
        "en": "Direction"
      },
      "rdfs:comment": {
        "en": "The class of table/text directions."
      }
    },
    {
      "@id": "csvw:Schema",
      "@type": "rdfs:Class",
      "rdfs:label": {
        "en": "Schema"
      },
      "rdfs:comment": {
        "en": "A Schema is a definition of a tabular format that may be common to multiple tables."
      }
    },
    {
      "@id": "csvw:Table",
      "@type": "rdfs:Class",
      "rdfs:label": {
        "en": "Table Description"
      },
      "rdfs:comment": {
        "en": "A Table describes an Annotated Table."
      }
    },
    {
      "@id": "csvw:TableGroup",
      "@type": "rdfs:Class",
      "rdfs:label": {
        "en": "Table Group Description"
      },
      "rdfs:comment": {
        "en": "A Table Group describes an Annotated Table Group."
      }
    },
    {
      "@id": "csvw:Template",
      "@type": "rdfs:Class",
      "rdfs:label": {
        "en": "Template Specification"
      },
      "rdfs:comment": {
        "en": "A Template Specification is a definition of how tabular data can be transformed into another format."
      }
    }
  ],
  "rdfs_properties": [
    {
      "@id": "csvw:aboutUrl",
      "@type": "rdf:Property",
      "rdfs:label": {
        "en": "about URL"
      },
      "rdfs:comment": {
        "en": "A URI template property that may be used to create a unique identifier for each cell within a row when mapping data to other formats"
      },
      "rdfs:domain": {
        "owl:unionOf": [
          "csvw:TableGroup",
          "csvw:Table",
          "csvw:Schema",
          "csvw:Column"
        ]
      },
      "rdfs:range": "csvw:uriTemplate"
    },
    {
      "@id": "csvw:columns",
      "@type": "rdf:Property",
      "rdfs:label": {
        "en": "columns"
      },
      "rdfs:comment": {
        "en": "An array of Column Descriptions."
      },
      "rdfs:domain": "csvw:Schema",
      "rdfs:range": "csvw:Column"
    },
    {
      "@id": "csvw:commentPrefix",
      "@type": "rdf:Property",
      "rdfs:label": {
        "en": "comment prefix"
      },
      "rdfs:comment": {
        "en": "A character that, when it appears at the beginning of a skipped row, indicates a comment that should be associated as a comment annotation to the table. The default is \"#\"."
      },
      "rdfs:domain": "csvw:Dialect",
      "rdfs:range": "xsd:string"
    },
    {
      "@id": "csvw:datatype",
      "@type": "rdf:Property",
      "rdfs:label": {
        "en": "datatype"
      },
      "rdfs:comment": {
        "en": "The main datatype of the values of the cell. If the cell contains a list (ie separator is specified and not null) then this is the datatype of each value within the list."
      },
      "rdfs:domain": {
        "owl:unionOf": [
          "csvw:TableGroup",
          "csvw:Table",
          "csvw:Schema",
          "csvw:Column"
        ]
      },
      "rdfs:range": "rdfs:Datatype"
    },
    {
      "@id": "csvw:default",
      "@type": "rdf:Property",
      "rdfs:label": {
        "en": "default"
      },
      "rdfs:comment": {
        "en": "An atomic property holding a single string that provides a default string value for the cell in cases where the original string value is a null value. This default value may be used when converting the table into other formats."
      },
      "rdfs:domain": {
        "owl:unionOf": [
          "csvw:TableGroup",
          "csvw:Table",
          "csvw:Schema",
          "csvw:Column"
        ]
      },
      "rdfs:range": "xsd:string"
    },
    {
      "@id": "csvw:delimiter",
      "@type": "rdf:Property",
      "rdfs:label": {
        "en": "delimiter"
      },
      "rdfs:comment": {
        "en": "The separator between cells. The default is \",\"."
      },
      "rdfs:domain": "csvw:Dialect",
      "rdfs:range": "xsd:string"
    },
    {
      "@id": "csvw:dialect",
      "@type": "rdf:Property",
      "rdfs:label": {
        "en": "dialect"
      },
      "rdfs:comment": {
        "en": "Provides hints to processors about how to parse the referenced files for to create tabular data models for an individual table, or all the tables in a group."
      },
      "rdfs:domain": {
        "owl:unionOf": [
          "csvw:TableGroup",
          "csvw:Table"
        ]
      },
      "rdfs:range": "csvw:Dialect"
    },
    {
      "@id": "csvw:doubleQuote",
      "@type": "rdf:Property",
      "rdfs:label": {
        "en": "double quote"
      },
      "rdfs:comment": {
        "en": "If true, sets the escape character flag to \". If false, to \\\\."
      },
      "rdfs:domain": "csvw:Dialect",
      "rdfs:range": "xsd:boolean"
    },
    {
      "@id": "csvw:encoding",
      "@type": "rdf:Property",
      "rdfs:label": {
        "en": "encoding"
      },
      "rdfs:comment": {
        "en": "The character encoding for the file, one of the encodings listed in [encoding]. The default is utf-8."
      },
      "rdfs:domain": "csvw:Dialect",
      "rdfs:range": "xsd:string"
    },
    {
      "@id": "csvw:foreignKeys",
      "@type": "rdf:Property",
      "rdfs:label": {
        "en": "foreign keys"
      },
      "rdfs:comment": {
        "en": "An array of foreign key definitions that define how the values from specified columns within this table link to rows within this table or other tables."
      },
      "rdfs:domain": "csvw:Schema",
      "rdfs:range": "xsd:string"
    },
    {
      "@id": "csvw:format",
      "@type": "rdf:Property",
      "rdfs:label": {
        "en": "format"
      },
      "rdfs:comment": {
        "en": "A definition of the format of the cell, used when parsing the cell."
      },
      "rdfs:domain": {
        "owl:unionOf": [
          "csvw:TableGroup",
          "csvw:Table",
          "csvw:Schema",
          "csvw:Column"
        ]
      },
      "rdfs:range": "xsd:string"
    },
    {
      "@id": "csvw:header",
      "@type": "rdf:Property",
      "rdfs:label": {
        "en": "header"
      },
      "rdfs:comment": {
        "en": ""
      },
      "rdfs:domain": "csvw:Dialect",
      "rdfs:range": "xsd:boolean"
    },
    {
      "@id": "csvw:headerColumnCount",
      "@type": "rdf:Property",
      "rdfs:label": {
        "en": "header column count"
      },
      "rdfs:comment": {
        "en": "The number of header columns (following the skipped columns) in each row. The default is 0.\n"
      },
      "rdfs:domain": "csvw:Dialect",
      "rdfs:range": "xsd:nonNegativeInteger"
    },
    {
      "@id": "csvw:headerRowCount",
      "@type": "rdf:Property",
      "rdfs:label": {
        "en": "header row count"
      },
      "rdfs:comment": {
        "en": "The number of header rows (following the skipped rows) in the file. The default is 1."
      },
      "rdfs:domain": "csvw:Dialect",
      "rdfs:range": "xsd:nonNegativeInteger"
    },
    {
      "@id": "csvw:language",
      "@type": "rdf:Property",
      "rdfs:label": {
        "en": "language"
      },
      "rdfs:comment": {
        "en": "A language code as defined by [BCP47]. Indicates the language of the value within the cell."
      },
      "rdfs:domain": {
        "owl:unionOf": [
          "csvw:TableGroup",
          "csvw:Table",
          "csvw:Schema",
          "csvw:Column"
        ]
      },
      "rdfs:range": "xsd:string"
    },
    {
      "@id": "csvw:length",
      "@type": "rdf:Property",
      "rdfs:label": {
        "en": "length"
      },
      "rdfs:comment": {
        "en": "The exact length of the value of the cell."
      },
      "rdfs:domain": {
        "owl:unionOf": [
          "csvw:TableGroup",
          "csvw:Table",
          "csvw:Schema",
          "csvw:Column"
        ]
      },
      "rdfs:range": "xsd:nonNegativeInteger"
    },
    {
      "@id": "csvw:lineTerminator",
      "@type": "rdf:Property",
      "rdfs:label": {
        "en": "line terminator"
      },
      "rdfs:comment": {
        "en": "The character that is used at the end of a row. The default is CRLF."
      },
      "rdfs:domain": "csvw:Dialect",
      "rdfs:range": "xsd:string"
    },
    {
      "@id": "csvw:maxExclusive",
      "@type": "rdf:Property",
      "rdfs:label": {
        "en": "max exclusive"
      },
      "rdfs:comment": {
        "en": "The maximum value for the cell (exclusive)."
      },
      "rdfs:domain": {
        "owl:unionOf": [
          "csvw:TableGroup",
          "csvw:Table",
          "csvw:Schema",
          "csvw:Column"
        ]
      },
      "rdfs:range": "xsd:integer"
    },
    {
      "@id": "csvw:maxInclusive",
      "@type": "rdf:Property",
      "rdfs:label": {
        "en": "max inclusive"
      },
      "rdfs:comment": {
        "en": "The maximum value for the cell (inclusive). "
      },
      "rdfs:domain": {
        "owl:unionOf": [
          "csvw:TableGroup",
          "csvw:Table",
          "csvw:Schema",
          "csvw:Column"
        ]
      },
      "rdfs:range": "xsd:integer"
    },
    {
      "@id": "csvw:maxLength",
      "@type": "rdf:Property",
      "rdfs:label": {
        "en": "max length"
      },
      "rdfs:comment": {
        "en": "The maximum length of the value of the cell."
      },
      "rdfs:domain": {
        "owl:unionOf": [
          "csvw:TableGroup",
          "csvw:Table",
          "csvw:Schema",
          "csvw:Column"
        ]
      },
      "rdfs:range": "xsd:nonNegativeInteger"
    },
    {
      "@id": "csvw:minExclusive",
      "@type": "rdf:Property",
      "rdfs:label": {
        "en": "min exclusive"
      },
      "rdfs:comment": {
        "en": "The minimum value for the cell (exclusive)."
      },
      "rdfs:domain": {
        "owl:unionOf": [
          "csvw:TableGroup",
          "csvw:Table",
          "csvw:Schema",
          "csvw:Column"
        ]
      },
      "rdfs:range": "xsd:integer"
    },
    {
      "@id": "csvw:minInclusive",
      "@type": "rdf:Property",
      "rdfs:label": {
        "en": "min inclusive"
      },
      "rdfs:comment": {
        "en": "The minimum value for the cell (inclusive)."
      },
      "rdfs:domain": {
        "owl:unionOf": [
          "csvw:TableGroup",
          "csvw:Table",
          "csvw:Schema",
          "csvw:Column"
        ]
      },
      "rdfs:range": "xsd:integer"
    },
    {
      "@id": "csvw:minLength",
      "@type": "rdf:Property",
      "rdfs:label": {
        "en": "min length"
      },
      "rdfs:comment": {
        "en": "The minimum length of the value of the cell."
      },
      "rdfs:domain": {
        "owl:unionOf": [
          "csvw:TableGroup",
          "csvw:Table",
          "csvw:Schema",
          "csvw:Column"
        ]
      },
      "rdfs:range": "xsd:nonNegativeInteger"
    },
    {
      "@id": "csvw:name",
      "@type": "rdf:Property",
      "rdfs:label": {
        "en": "name"
      },
      "rdfs:comment": {
        "en": "An atomic property that gives a canonical name for the column. This must be a string. Conversion specifications must use this property as the basis for the names of properties/elements/attributes in the results of conversions."
      },
      "rdfs:domain": "csvw:Column",
      "rdfs:range": "xsd:string"
    },
    {
      "@id": "csvw:notes",
      "@type": "rdf:Property",
      "rdfs:label": {
        "en": "notes"
      },
      "rdfs:comment": {
        "en": "An array of objects representing annotations. This specification does not place any constraints on the structure of these objects."
      },
      "rdfs:domain": "csvw:Table"
    },
    {
      "@id": "csvw:null",
      "@type": "rdf:Property",
      "rdfs:label": {
        "en": "null"
      },
      "rdfs:comment": {
        "en": "The string used for null values. If not specified, the default for this is the empty string."
      },
      "rdfs:domain": {
        "owl:unionOf": [
          "csvw:TableGroup",
          "csvw:Table",
          "csvw:Schema",
          "csvw:Column"
        ]
      },
      "rdfs:range": "xsd:string"
    },
    {
      "@id": "csvw:primaryKey",
      "@type": "rdf:Property",
      "rdfs:label": {
        "en": "primary key"
      },
      "rdfs:comment": {
        "en": "A column reference property that holds either a single reference to a column description object or an array of references."
      },
      "rdfs:domain": "csvw:Schema",
      "rdfs:range": "xsd:string"
    },
    {
      "@id": "csvw:propertyUrl",
      "@type": "rdf:Property",
      "rdfs:label": {
        "en": "property URL"
      },
      "rdfs:comment": {
        "en": "An URI template property that holds one or more strings that may be expanded to URIs for properties if the table is mapped to another format. The default value of propertyUrl is \"{#_name}\"."
      },
      "rdfs:domain": {
        "owl:unionOf": [
          "csvw:TableGroup",
          "csvw:Table",
          "csvw:Schema",
          "csvw:Column"
        ]
      },
      "rdfs:range": "csvw:uriTemplate"
    },
    {
      "@id": "csvw:quoteChar",
      "@type": "rdf:Property",
      "rdfs:label": {
        "en": "quote char"
      },
      "rdfs:comment": {
        "en": "The character that is used around escaped cells."
      },
      "rdfs:domain": "csvw:Dialect",
      "rdfs:range": "xsd:string"
    },
    {
      "@id": "csvw:required",
      "@type": "rdf:Property",
      "rdfs:label": {
        "en": "required"
      },
      "rdfs:comment": {
        "en": "A boolean value which indicates whether every cell within the column must have a non-null value."
      },
      "rdfs:domain": "csvw:Column",
      "rdfs:range": "xsd:boolean"
    },
    {
      "@id": "csvw:resources",
      "@type": "rdf:Property",
      "rdfs:label": {
        "en": "resources"
      },
      "rdfs:comment": {
        "en": "An array of table descriptions for the tables in the group."
      },
      "rdfs:domain": "csvw:TableGroup",
      "rdfs:range": "csvw:Table"
    },
    {
      "@id": "csvw:row",
      "@type": "rdf:Property",
      "rdfs:label": {
        "en": "row"
      },
      "rdfs:comment": {
        "en": "Relates a Table to each Row output."
      },
      "rdfs:subPropertyOf": "rdfs:member",
      "rdfs:domain": "csvw:Table"
    },
    {
      "@id": "csvw:separator",
      "@type": "rdf:Property",
      "rdfs:label": {
        "en": "separator"
      },
      "rdfs:comment": {
        "en": "The character used to separate items in the string value of the cell."
      },
      "rdfs:domain": {
        "owl:unionOf": [
          "csvw:TableGroup",
          "csvw:Table",
          "csvw:Schema",
          "csvw:Column"
        ]
      },
      "rdfs:range": "xsd:string"
    },
    {
      "@id": "csvw:skipBlankRows",
      "@type": "rdf:Property",
      "rdfs:label": {
        "en": "skip blank rows"
      },
      "rdfs:comment": {
        "en": "Indicates whether to ignore wholly empty rows (ie rows in which all the cells are empty). The default is false."
      },
      "rdfs:domain": "csvw:Dialect",
      "rdfs:range": "xsd:boolean"
    },
    {
      "@id": "csvw:skipColumns",
      "@type": "rdf:Property",
      "rdfs:label": {
        "en": "skip columns"
      },
      "rdfs:comment": {
        "en": "The number of columns to skip at the beginning of each row, before any header columns. The default is 0."
      },
      "rdfs:domain": "csvw:Dialect",
      "rdfs:range": "xsd:nonNegativeInteger"
    },
    {
      "@id": "csvw:skipInitialSpace",
      "@type": "rdf:Property",
      "rdfs:label": {
        "en": "skip initial space"
      },
      "rdfs:comment": {
        "en": "If true, sets the trim flag to \"start\". If false, to false."
      },
      "rdfs:domain": "csvw:Dialect",
      "rdfs:range": "xsd:boolean"
    },
    {
      "@id": "csvw:skipRows",
      "@type": "rdf:Property",
      "rdfs:label": {
        "en": "skip rows"
      },
      "rdfs:comment": {
        "en": "The number of rows to skip at the beginning of the file, before a header row or tabular data."
      },
      "rdfs:domain": "csvw:Dialect",
      "rdfs:range": "xsd:nonNegativeInteger"
    },
    {
      "@id": "csvw:source",
      "@type": "rdf:Property",
      "rdfs:label": {
        "en": "source"
      },
      "rdfs:comment": {
        "en": "The format to which the tabular data should be transformed prior to the transformation using the template. If the value is \"json\", the tabular data should first be transformed first to JSON based on the simple mapping defined in Generating JSON from Tabular Data on the Web. If the value is \"rdf\", it should similarly first be transformed to XML based on the simple mapping defined in Generating RDF from Tabular Data on the Web."
      },
      "rdfs:domain": "csvw:Template",
      "rdfs:range": "xsd:string"
    },
    {
      "@id": "csvw:table",
      "@type": "rdf:Property",
      "rdfs:label": {
        "en": "table"
      },
      "rdfs:comment": {
        "en": "Relates an Table group to annotated tables. (Note, this is different from csvw:resources, which relates metadata, rather than resulting annotated table descriptions."
      },
      "rdfs:subPropertyOf": "rdfs:member",
      "rdfs:domain": "csvw:TableGroup",
      "rdfs:range": "csvw:Table"
    },
    {
      "@id": "csvw:tableDirection",
      "@type": "rdf:Property",
      "rdfs:label": {
        "en": "table direction"
      },
      "rdfs:comment": {
        "en": "One of csvw:rtl csvw:ltr or csvw:default. Indicates whether the tables in the group should be displayed with the first column on the right, on the left, or based on the first character in the table that has a specific direction. "
      },
      "rdfs:domain": {
        "owl:unionOf": [
          "csvw:TableGroup",
          "csvw:Table"
        ]
      },
      "rdfs:range": "csvw:Direction"
    },
    {
      "@id": "csvw:tableSchema",
      "@type": "rdf:Property",
      "rdfs:label": {
        "en": "table schema"
      },
      "rdfs:comment": {
        "en": "An object property that provides a schema description for an individual table, or all the tables in a group."
      },
      "rdfs:domain": {
        "owl:unionOf": [
          "csvw:TableGroup",
          "csvw:Table"
        ]
      },
      "rdfs:range": "csvw:Schema"
    },
    {
      "@id": "csvw:targetFormat",
      "@type": "rdf:Property",
      "rdfs:label": {
        "en": "target format"
      },
      "rdfs:comment": {
        "en": "A URL for the format that will be created through the transformation. If one has been defined, this should be a URL for a media type, in the form http://www.iana.org/assignments/media-types/media-type such as http://www.iana.org/assignments/media-types/text/calendar. Otherwise, it can be any URL that describes the target format."
      },
      "rdfs:domain": "csvw:Template",
      "rdfs:range": "xsd:anyURI"
    },
    {
      "@id": "csvw:templateFormat",
      "@type": "rdf:Property",
      "rdfs:label": {
        "en": "template format"
      },
      "rdfs:comment": {
        "en": "A URL for the format that is used by the template. If one has been defined, this should be a URL for a media type, in the form http://www.iana.org/assignments/media-types/media-type such as http://www.iana.org/assignments/media-types/application/javascript. Otherwise, it can be any URL that describes the template format."
      },
      "rdfs:domain": "csvw:Template",
      "rdfs:range": "xsd:anyURI"
    },
    {
      "@id": "csvw:templates",
      "@type": "rdf:Property",
      "rdfs:label": {
        "en": "templates"
      },
      "rdfs:comment": {
        "en": "An array of template specifications that provide mechanisms to transform the tabular data into other formats. "
      },
      "rdfs:domain": {
        "owl:unionOf": [
          "csvw:TableGroup",
          "csvw:Table"
        ]
      },
      "rdfs:range": "csvw:Template"
    },
    {
      "@id": "csvw:textDirection",
      "@type": "rdf:Property",
      "rdfs:label": {
        "en": "text direction"
      },
      "rdfs:comment": {
        "en": "One of csvw:rtl or csvw:ltr. Indicates whether the text within cells should be displayed by default as left-to-right or right-to-left text. "
      },
      "rdfs:domain": {
        "owl:unionOf": [
          "csvw:TableGroup",
          "csvw:Table",
          "csvw:Schema",
          "csvw:Column"
        ]
      },
      "rdfs:range": "csvw:Direction"
    },
    {
      "@id": "csvw:title",
      "@type": "rdf:Property",
      "rdfs:label": {
        "en": "title"
      },
      "rdfs:comment": {
        "en": "For a Template: A natural language property that describes the format that will be generated from the transformation. This is useful if the target format is a generic format (such as application/json) and the transformation is creating a specific profile of that format.\n\nFor a Column: A natural language property that provides possible alternative names for the column."
      },
      "rdfs:domain": {
        "owl:unionOf": [
          "csvw:Template",
          "csvw:Column"
        ]
      }
    },
    {
      "@id": "csvw:trim",
      "@type": "rdf:Property",
      "rdfs:label": {
        "en": "trim"
      },
      "rdfs:comment": {
        "en": "Indicates whether to trim whitespace around cells; may be true, false, start or end. The default is false."
      },
      "rdfs:domain": "csvw:Dialect",
      "rdfs:range": "xsd:boolean"
    },
    {
      "@id": "csvw:url",
      "@type": "rdf:Property",
      "rdfs:label": {
        "en": "url"
      },
      "rdfs:comment": {
        "en": "For a Table: This link property gives the single URL of the CSV file that the table is held in, relative to the location of the metadata document.\n\nFor a Template: A link property giving the single URL of the file that the template is held in, relative to the location of the metadata document."
      },
      "rdfs:domain": {
        "owl:unionOf": [
          "csvw:Table",
          "csvw:Template"
        ]
      },
      "rdfs:range": "xsd:anyURI"
    },
    {
      "@id": "csvw:valueUrl",
      "@type": "rdf:Property",
      "rdfs:label": {
        "en": "valueUrl"
      },
      "rdfs:comment": {
        "en": "An URI template property that is used to define one or more resources value of a cell instead of a literal values."
      },
      "rdfs:domain": {
        "owl:unionOf": [
          "csvw:TableGroup",
          "csvw:Table",
          "csvw:Schema",
          "csvw:Column"
        ]
      },
      "rdfs:range": "csvw:uriTemplate"
    },
    {
      "@id": "csvw:virtual",
      "@type": "rdf:Property",
      "rdfs:label": {
        "en": "virtual"
      },
      "rdfs:comment": {
        "en": "A boolean atomic property taking a single value which indicates whether the column is a virtual column not present in the original source"
      },
      "rdfs:domain": "csvw:Column",
      "rdfs:range": "xsd:boolean"
    }
  ],
  "rdfs_datatypes": [
    {
      "@id": "csvw:JSON",
      "@type": "rdfs:Datatype",
      "rdfs:label": {
        "en": "JSON"
      },
      "rdfs:comment": {
        "en": "A literal containing JSON."
      },
      "rdfs:subClassOf": "xsd:string"
    },
    {
      "@id": "csvw:uriTemplate",
      "@type": "rdfs:Datatype",
      "rdfs:label": {
        "en": "uri template"
      },
      "rdfs:comment": {
        "en": ""
      },
      "rdfs:subClassOf": "xsd:anyURI"
    }
  ],
  "rdfs_instances": [
    {
      "@id": "csvw:ltr",
      "@type": "Direction",
      "rdfs:label": {
        "en": "left to right"
      },
      "rdfs:comment": {
        "en": "Indicates text should be processed left to right."
      }
    },
    {
      "@id": "csvw:rtl",
      "@type": "Direction",
      "rdfs:label": {
        "en": "right to left"
      },
      "rdfs:comment": {
        "en": "Indiects text should be processed right to left"
      }
    },
    {
      "@id": "csvw:csvEncodedTabularData",
      "@type": "prov:Role",
      "rdfs:label": {
        "en": "CSV Encoded Tabular Data"
      },
      "rdfs:comment": {
        "en": "Describes the role of a CSV file in the tabular data mapping."
      }
    },
    {
      "@id": "csvw:tabularMetadata",
      "@type": "prov:Role",
      "rdfs:label": {
        "en": "Tabular Metadata"
      },
      "rdfs:comment": {
        "en": "Describes the role of a Metadata file in the tabular data mapping."
      }
    }
  ]
}
